add type elaboration and soundness proof

TabularTypeInterpreter/Semantics.lean
@@ -1,3 +1,4 @@
+import Lott.DSL.Elab.UniversalJudgement
 import TabularTypeInterpreter.Syntax
 import TabularTypeInterpreter.«F⊗⊕ω»
 
@@ -29,5 +30,881 @@ judgement Kind.Elaboration :=
 
 ─────── constr
 ⊢ C ⇝ *
+
+instance : Coe TypeVarId «F⊗⊕ω».TypeVarId where coe a := a
+
+instance : Coe TypeVarId «F⊗⊕ω».TypeVar where coe a := .free a
+
+judgement_syntax a " : " κ " ∈ " Γ : TypeEnvironment.TypeVarIn (id a)
+
+judgement TypeEnvironment.TypeVarIn :=
+
+──────────────── head
+a : κ ∈ Γ, a : κ
+
+a ≠ a'
+a : κ ∈ Γ
+────────────────── typeExt
+a : κ ∈ Γ, a' : κ'
+
+a : κ ∈ Γ
+──────────────── termExt
+a : κ ∈ Γ, x : σ
+
+a : κ ∈ Γ
+──────────────── constrExt
+a : κ ∈ Γ, ψ ⇝ x
+
+judgement_syntax ℓ " ≠ " ℓ' : Label.Ne
+
+def Label.Ne := _root_.Ne (α := Label)
+
+judgement_syntax "unique" "(" sepBy(ξ, ", ") ")" : Monotype.label.Uniqueness
+
+judgement Monotype.label.Uniqueness :=
+
+</ </ ℓ@i ≠ ℓ@j // j ∈ [i + 1:n] /> // i ∈ [:n] />
+────────────────────────────────────────────────── concrete
+unique(</ ℓ@i // i ∈ [:n] />)
+
+───────── var
+unique(ξ)
+
+judgement_syntax TC " ≠ " TC' : TypeClass.Ne
+
+def TypeClass.Ne := _root_.Ne (α := TypeClass)
+
+judgement_syntax m " ≠ " m' : Member.Ne
+
+def Member.Ne := _root_.Ne (α := Member)
+
+judgement_syntax γc " ∈ " Γc : ClassEnvironment.In
+
+judgement ClassEnvironment.In :=
+
+─────────── head
+γc ∈ Γc, γc
+
+(</ TCₛ@i a ⇝ Aₛ@i // i ∈ [:n] /> ⇒ TC a : κ) ↦ m : σ ⇝ A ∈ Γc
+TC ≠ TC'
+m ≠ m'
+────────────────────────────────────────────────────────────────────────────────────────────────────────────────────────────────── ext {TC}
+(</ TCₛ@i a ⇝ Aₛ@i // i ∈ [:n] /> ⇒ TC a : κ) ↦ m : σ ⇝ A ∈ Γc, (</ TC'ₛ@i a' ⇝ Aₛ'@i // i ∈ [:m] /> ⇒ TC' a' : κ') ↦ m' : σ' ⇝ A'
+
+def TypeEnvironment.typeVarDom : TypeEnvironment → List TypeVarId
+  | .empty => []
+  | .typeExt Γ a _ => a :: Γ.typeVarDom
+  | .termExt Γ .. => Γ.typeVarDom
+  | .constrExt Γ .. => Γ.typeVarDom
+
+def TypeEnvironment.termVarDom : TypeEnvironment → List TermVarId
+  | .empty => []
+  | .typeExt Γ .. => Γ.termVarDom
+  | .termExt Γ x _ => x :: Γ.termVarDom
+  | .constrExt Γ _ x => x :: Γ.termVarDom
+
+judgement_syntax a " ∉ " "dom" "(" Γ ")" : TypeEnvironment.TypeVarNotInDom (id a)
+
+def TypeEnvironment.TypeVarNotInDom a (Γ : TypeEnvironment) := a ∉ Γ.typeVarDom
+
+instance : Coe TermVarId «F⊗⊕ω».TermVarId where coe x := x
+
+judgement_syntax x " ∉ " "dom'" "(" Γ ")" : TypeEnvironment.TermVarNotInDom (id x)
+
+def TypeEnvironment.TermVarNotInDom x (Γ : TypeEnvironment) := x ∉ Γ.termVarDom
+
+judgement_syntax Γc "; " Γ " ⊢ " σ " : " κ " ⇝ " A : TypeScheme.KindingAndElaboration
+
+judgement_syntax Γc " ⊢ " Γ " ⇝ " Δ : TypeEnvironment.WellFormednessAndElaboration
+
+judgement_syntax "⊢c " Γc : ClassEnvironment.WellFormedness
+
+mutual
+
+judgement TypeScheme.KindingAndElaboration :=
+
+a : κ ∈ Γ
+───────────────── var
+Γc; Γ ⊢ a : κ ⇝ a
+
+Γc; Γ ⊢ φ : κ₀ ↦ κ₁ ⇝ A
+Γc; Γ ⊢ τ : κ₀ ⇝ B
+─────────────────────── app
+Γc; Γ ⊢ φ τ : κ₁ ⇝ A B
+
+Γc; Γ ⊢ τ₀ : * ⇝ A
+Γc; Γ ⊢ τ₁ : * ⇝ B
+─────────────────────────── arr
+Γc; Γ ⊢ τ₀ → τ₁ : * ⇝ A → B
+
+Γc; Γ ⊢ ψ : C ⇝ A
+Γc; Γ ⊢ γ : κ ⇝ B
+⊢ κ ⇝ *
+───────────────────────── qual
+Γc; Γ ⊢ ψ ⇒ γ : κ ⇝ A → B
+
+∀ a ∉ I, Γc; Γ, a : κ₀ ⊢ σ^a : κ₁ ⇝ A^a
+⊢ κ₀ ⇝ K₀
+─────────────────────────────────────── scheme (I : List TypeVarId)
+Γc; Γ ⊢ ∀ a : κ₀. σ : κ₁ ⇝ ∀ a : K₀. A
+
+───────────────────── label
+Γc; Γ ⊢ ℓ : L ⇝ ⊗ { }
+
+Γc; Γ ⊢ ξ : L ⇝ A
+─────────────────────── floor
+Γc; Γ ⊢ ⌊ξ⌋ : * ⇝ ⊗ { }
+
+───────────────────── comm
+Γc; Γ ⊢ u : U ⇝ ⊗ { }
+
+</ Γc; Γ ⊢ ξ@i : L ⇝ B@i // i ∈ [:n] />
+unique(</ ξ@i // i ∈ [:n] />)
+</ Γc; Γ ⊢ τ@i : κ ⇝ A@i // i ∈ [:n] />
+───────────────────────────────────────────────────────────────────── row
+Γc; Γ ⊢ ⟨</ ξ@i ▹ τ@i // i ∈ [:n] />⟩ : R κ ⇝ {</ A@i // i ∈ [:n] />}
+
+Γc; Γ ⊢ μ : U ⇝ B
+Γc; Γ ⊢ ρ : R * ⇝ A
+──────────────────────── prod
+Γc; Γ ⊢ Π(μ) ρ : * ⇝ ⊗ A
+
+Γc; Γ ⊢ μ : U ⇝ B
+Γc; Γ ⊢ ρ : R * ⇝ A
+──────────────────────── sum
+Γc; Γ ⊢ Σ(μ) ρ : * ⇝ ⊕ A
+
+∀ a ∉ I, Γc; Γ, a : κ₀ ⊢ τ^a : κ₁ ⇝ A^a
+⊢ κ₀ ⇝ K₀
+Γc; Γ ⊢ ρ : R κ₀ ⇝ B
+─────────────────────────────────────────────────────── lift (I : List TypeVarId)
+Γc; Γ ⊢ Lift (λ a : κ₀. τ) ρ : R κ₁ ⇝ (λ a : K₀. A) ⟦B⟧
+
+Γc; Γ ⊢ μ : U ⇝ B
+Γc; Γ ⊢ ρ₀ : R κ ⇝ A₀
+Γc; Γ ⊢ ρ₁ : R κ ⇝ A₁
+⊢ κ ⇝ K
+─────────────────────────────────────────────────────────────────────────────────────────────────────────────────── contain
+Γc; Γ ⊢ ρ₀ ≲(μ) ρ₁ : C ⇝ ⊗ {∀ a : K ↦ *. (⊗ (a$0 ⟦A₁⟧)) → ⊗ (a$0 ⟦A₀⟧), ∀ a : K ↦ *. (⊕ (a$0 ⟦A₀⟧)) → ⊕ (a$0 ⟦A₁⟧)}
+
+Γc; Γ ⊢ μ : U ⇝ B
+Γc; Γ ⊢ ρ₀ : R κ ⇝ A₀
+Γc; Γ ⊢ ρ₁ : R κ ⇝ A₁
+Γc; Γ ⊢ ρ₂ : R κ ⇝ A₂
+⊢ κ ⇝ K
+Γc; Γ ⊢ ρ₀ ≲(μ) ρ₂ : C ⇝ Bₗ
+Γc; Γ ⊢ ρ₁ ≲(μ) ρ₂ : C ⇝ Bᵣ
+─────────────────────────────────────────────────────────────────────────────────────────────────────────────────────────────────────────────────────────────────────────────────────────────────────── concat
+Γc; Γ ⊢ ρ₀ ⊙(μ) ρ₁ ~ ρ₂ : C ⇝ ⊗ {∀ a : K ↦ *. (⊗ (a$0 ⟦A₀⟧)) → (⊗ (a$0 ⟦A₁⟧)) → ⊗ (a$0 ⟦A₂⟧), ∀ a : K ↦ *. ∀ aₜ : *. ((⊕ (a$1 ⟦A₀⟧)) → aₜ$0) → ((⊕ (a$1 ⟦A₁⟧)) → aₜ$0) → (⊕ (a$1 ⟦A₂⟧)) → aₜ$0, Bₗ, Bᵣ}
+
+⊢c Γc
+(</ TCₛ@i a ⇝ Aₛ@i // i ∈ [:n] /> ⇒ TC a : κ) ↦ m : σ ⇝ A ∈ Γc
+Γc; Γ ⊢ τ : κ ⇝ B
+────────────────────────────────────────────────────────────── tc {TC}
+Γc; Γ ⊢ TC τ : C ⇝ ⊗ {A^^B, </ Aₛ@i^^B // i ∈ [:n] /> }
+
+∀ a ∉ I, Γc; Γ, a : κ ⊢ ψ^a : C ⇝ A^a
+⊢ κ ⇝ K
+Γc; Γ ⊢ ρ : R κ ⇝ B
+───────────────────────────────────────────────────── all (I : List TypeVarId)
+Γc; Γ ⊢ All (λ a : κ. ψ) ρ : C ⇝ ⊗ ((λ a : K. A) ⟦B⟧)
+
+Γc; Γ ⊢ ρ : R κ ⇝ A
+⊢ κ ⇝ K
+∀ aₗ ∉ I₀, ∀ aₜ ∉ aₗ :: I₀, ∀ aₚ ∉ aₜ :: aₗ :: I₀, ∀ aᵢ ∉ aₚ :: aₜ :: aₗ :: I₀, ∀ aₙ ∉ aᵢ :: aₚ :: aₜ :: aₗ :: I₀, Γc; Γ, aₗ : L, aₜ : κ, aₚ : R κ, aᵢ : R κ, aₙ : R κ ⊢ ⟨aₗ ▹ aₜ⟩ ⊙(N) aₚ ~ aᵢ : C ⇝ Bᵣ^aₙ^aᵢ^aₚ^aₜ^aₗ
+∀ aᵢ ∉ I₁, ∀ aₙ ∉ aᵢ :: I₁, Γc; Γ, aᵢ : R κ, aₙ : R κ ⊢ aᵢ ⊙(N) aₙ ~ ρ : C ⇝ Bₗ^aₙ^aᵢ
+─────────────────────────────────────────────────────────────────────────────────────────────────────────────────────────────────────────────────────────────────────────────────────────────────────────────────────── ind (I₀ I₁)
+Γc; Γ ⊢ Ind ρ : C ⇝ ∀ aₘ : (L K) ↦ *. (∀ aₗ : *. ∀ aₜ : K. ∀ aₚ : L K. ∀ aᵢ : L K. ∀ aₙ : L K. Bᵣ → Bₗ → aₗ$4 → aₘ$5 aₚ$2 → aₘ$5 aₙ$0) → aₘ$5 { } → aₘ$5 A
+
+Γc; Γ ⊢ (Lift (λ a : *. τ) ρ₀) ⊙(C) ρ₁ ~ ρ₂ : C ⇝ A
+─────────────────────────────────────────────────── split
+Γc; Γ ⊢ Split (λ a : *. τ) ρ₀ ⊙' ρ₁ ~ ρ₂ : C ⇝ A
+
+judgement TypeEnvironment.WellFormednessAndElaboration :=
+
+────────── empty
+Γc ⊢ ε ⇝ ε
+
+Γc ⊢ Γ ⇝ Δ
+a ∉ dom(Γ)
+⊢ κ ⇝ K
+──────────────────────── typeExt
+Γc ⊢ Γ, a : κ ⇝ Δ, a : K
+
+Γc ⊢ Γ ⇝ Δ
+x ∉ dom'(Γ)
+Γc; Γ ⊢ σ : * ⇝ A
+──────────────────────── termExt
+Γc ⊢ Γ, x : σ ⇝ Δ, x : A
+
+Γc ⊢ Γ ⇝ Δ
+x ∉ dom'(Γ)
+Γc; Γ ⊢ ψ : C ⇝ A
+──────────────────────── constrExt
+Γc ⊢ Γ, ψ ⇝ x ⇝ Δ, x : A
+
+judgement ClassEnvironment.WellFormedness :=
+
+──── empty
+⊢c ε
+
+⊢c Γc
+⊢ κ ⇝ K
+∀ a, Γc; ε, a : κ ⊢ σ : * ⇝ A^a
+∀ a, ε, a : K ⊢ A^a : *
+</ ∀ a, Γc; ε, a : κ ⊢ TCₛ@i a : * ⇝ Aₛ@i^a // i ∈ [:n] />
+</ ∀ a, ε, a : K ⊢ Aₛ@i^a : * // i ∈ [:n] />
+──────────────────────────────────────────────────────────────── ext {TC}
+⊢c Γc, (</ TCₛ@i a ⇝ Aₛ@i // i ∈ [:n] /> ⇒ TC a : κ) ↦ m : σ ⇝ A
+
+end
+
+namespace Kind
+
+theorem Elaboration_total (κ : Kind) : ∃ K, [[⊢ κ ⇝ K]] := match κ with
+  | .star => .intro _ .star
+  | .arr κ₀ κ₁ =>
+    let ⟨_, κ₀e⟩ := κ₀.Elaboration_total
+    let ⟨_, κ₁e⟩ := κ₁.Elaboration_total
+    .intro _ <| .arr κ₀e κ₁e
+  | .label => .intro _ .label
+  | .comm => .intro _ .comm
+  | .row κ =>
+    let ⟨_, κe⟩ := κ.Elaboration_total
+    .intro _ <| .row κe
+  | .constr => .intro _ .constr
+
+theorem Elaboration.deterministic (κe₀ : [[⊢ κ ⇝ K₀]]) (κe₁ : [[⊢ κ ⇝ K₁]]) : K₀ = K₁ :=
+  match κ, κe₀, κe₁ with
+  | .star, .star, .star => rfl
+  | .arr _ _, .arr κ₀e κ₁e, .arr κ₀e' κ₁e' =>
+    let .refl _ := κ₀e.deterministic κ₀e'
+    let .refl _ := κ₁e.deterministic κ₁e'
+    rfl
+  | .label, .label, .label => rfl
+  | .comm, .comm, .comm => rfl
+  | .row _, .row κ'e, .row κ'e' => let .refl _ := κ'e.deterministic κ'e'; rfl
+  | .constr, .constr, .constr => rfl
+
+end Kind
+
+theorem TypeEnvironment.WellFormednessAndElaboration.TypeVarIn_preservation (Γwe : [[Γc ⊢ Γ ⇝ Δ]])
+  (aκinΓ : [[a : κ ∈ Γ]]) (κe : [[⊢ κ ⇝ K]]) : [[a : K ∈ Δ]] :=
+  match Γwe, aκinΓ with
+  | .typeExt _ _ κe' (K := K'), .head => let .refl _ := κe.deterministic κe'; .head
+  | .typeExt Γ'we _ _ (a := a') , .typeExt anea'' aκinΓ' =>
+    Γ'we.TypeVarIn_preservation aκinΓ' κe |>.typeVarExt anea''
+  | .termExt Γ'we .., .termExt aκinΓ' => Γ'we.TypeVarIn_preservation aκinΓ' κe |>.termVarExt
+  | .constrExt Γ'we .., .constrExt aκinΓ' => Γ'we.TypeVarIn_preservation aκinΓ' κe |>.termVarExt
+
+namespace «F⊗⊕ω».Kinding
+
+theorem unit : [[Δ ⊢ ⊗ { } : *]] := by
+  have := list (Δ := Δ) (A := fun _ => .list []) (K := .star) (n := 0) (fun _ => nomatch ·)
+  simp [Coe.coe, Std.Range.toList] at this
+  exact prod this
+
+theorem prj_evidence (Δwf : [[⊢ Δ]]) (A₀ki : [[Δ ⊢ A₀ : L K]]) (A₁ki : [[Δ ⊢ A₁ : L K]])
+  : [[Δ ⊢ ∀ a : K ↦ *. (⊗ (a$0 ⟦A₁⟧)) → ⊗ (a$0 ⟦A₀⟧) : *]] := by
+  apply scheme (I := Δ.typeVarDom)
+  intro a anin
+  simp [«Type».TypeVar_open]
+  apply arr
+  · apply prod
+    apply listApp
+    · exact var .head
+    · rw [A₁ki.TypeVarLocallyClosed_of.TypeVar_open_eq, ← Δ.empty_append]
+      apply A₁ki.weakening (Δ' := .empty) (Δ'' := .typeExt .empty a _)
+      rw [Environment.empty_append]
+      exact Δwf.typeVarExt anin
+  · apply prod
+    apply listApp
+    · exact var .head
+    · rw [A₀ki.TypeVarLocallyClosed_of.TypeVar_open_eq, ← Δ.empty_append]
+      apply A₀ki.weakening (Δ' := .empty) (Δ'' := .typeExt .empty a _)
+      rw [Environment.empty_append]
+      exact Δwf.typeVarExt anin
+
+theorem inj_evidence (Δwf : [[⊢ Δ]]) (A₀ki : [[Δ ⊢ A₀ : L K]]) (A₁ki : [[Δ ⊢ A₁ : L K]])
+  : [[Δ ⊢ ∀ a : K ↦ *. (⊕ (a$0 ⟦A₀⟧)) → ⊕ (a$0 ⟦A₁⟧) : *]] := by
+  apply scheme (I := Δ.typeVarDom)
+  intro a anin
+  simp only [«Type».TypeVar_open]
+  apply arr
+  · apply sum
+    apply listApp
+    · exact var .head
+    · rw [A₀ki.TypeVarLocallyClosed_of.TypeVar_open_eq, ← Δ.empty_append]
+      apply A₀ki.weakening (Δ' := .empty) (Δ'' := .typeExt .empty a _)
+      rw [Environment.empty_append]
+      exact Δwf.typeVarExt anin
+  · apply sum
+    apply listApp
+    · exact var .head
+    · rw [A₁ki.TypeVarLocallyClosed_of.TypeVar_open_eq, ← Δ.empty_append]
+      apply A₁ki.weakening (Δ' := .empty) (Δ'' := .typeExt .empty a _)
+      rw [Environment.empty_append]
+      exact Δwf.typeVarExt anin
+
+theorem concat_evidence (Δwf : [[⊢ Δ]]) (A₀ki : [[Δ ⊢ A₀ : L K]]) (A₁ki : [[Δ ⊢ A₁ : L K]])
+  (A₂ki : [[Δ ⊢ A₂ : L K]])
+  : [[Δ ⊢ ∀ a : K ↦ *. (⊗ (a$0 ⟦A₀⟧)) → (⊗ (a$0 ⟦A₁⟧)) → ⊗ (a$0 ⟦A₂⟧) : *]] := by
+  apply scheme (I := Δ.typeVarDom)
+  intro a anin
+  simp only [«Type».TypeVar_open]
+  apply arr
+  · apply prod
+    apply listApp
+    · exact var .head
+    · rw [A₀ki.TypeVarLocallyClosed_of.TypeVar_open_eq, ← Δ.empty_append]
+      apply A₀ki.weakening (Δ' := .empty) (Δ'' := .typeExt .empty a _)
+      rw [Environment.empty_append]
+      exact Δwf.typeVarExt anin
+  · apply arr
+    · apply prod
+      apply listApp
+      · exact var .head
+      · rw [A₁ki.TypeVarLocallyClosed_of.TypeVar_open_eq, ← Δ.empty_append]
+        apply A₁ki.weakening (Δ' := .empty) (Δ'' := .typeExt .empty a _)
+        rw [Environment.empty_append]
+        exact Δwf.typeVarExt anin
+    · apply prod
+      apply listApp
+      · exact var .head
+      · rw [A₂ki.TypeVarLocallyClosed_of.TypeVar_open_eq, ← Δ.empty_append]
+        apply A₂ki.weakening (Δ' := .empty) (Δ'' := .typeExt .empty a _)
+        rw [Environment.empty_append]
+        exact Δwf.typeVarExt anin
+
+theorem elim_evidence (Δwf : [[⊢ Δ]]) (A₀ki : [[Δ ⊢ A₀ : L K]]) (A₁ki : [[Δ ⊢ A₁ : L K]])
+  (A₂ki : [[Δ ⊢ A₂ : L K]])
+  : [[Δ ⊢ ∀ a : K ↦ *. ∀ aₜ : *. ((⊕ (a$1 ⟦A₀⟧)) → aₜ$0) → ((⊕ (a$1 ⟦A₁⟧)) → aₜ$0) → (⊕ (a$1 ⟦A₂⟧)) → aₜ$0 : *]] := by
+  apply scheme (I := Δ.typeVarDom)
+  intro a anin
+  simp [«Type».TypeVar_open]
+  apply scheme (I := a :: Δ.typeVarDom)
+  intro aₜ aₜnin
+  let aₜnea := List.ne_of_not_mem_cons aₜnin
+  simp [«Type».TypeVar_open]
+  apply arr
+  · apply arr
+    · apply sum
+      apply listApp
+      · exact var <| .typeVarExt .head aₜnea.symm
+      · let A₀lc := A₀ki.TypeVarLocallyClosed_of
+        rw [A₀lc.weaken (n := 1) |>.TypeVar_open_eq, A₀lc.TypeVar_open_eq, ← Δ.empty_append]
+        apply A₀ki.weakening (Δ' := .empty) (Δ'' := .typeExt (.typeExt .empty a _) aₜ _)
+        rw [Environment.empty_append]
+        exact Δwf.typeVarExt anin |>.typeVarExt aₜnin
+    · exact var .head
+  · apply arr
+    · apply arr
+      · apply sum
+        apply listApp
+        · exact var <| .typeVarExt .head aₜnea.symm
+        · let A₁lc := A₁ki.TypeVarLocallyClosed_of
+          rw [A₁lc.weaken (n := 1) |>.TypeVar_open_eq, A₁lc.TypeVar_open_eq, ← Δ.empty_append]
+          apply A₁ki.weakening (Δ' := .empty) (Δ'' := .typeExt (.typeExt .empty a _) aₜ _)
+          rw [Environment.empty_append]
+          exact Δwf.typeVarExt anin |>.typeVarExt aₜnin
+      · exact var .head
+    · apply arr
+      · apply sum
+        apply listApp
+        · exact var <| .typeVarExt .head aₜnea.symm
+        · let A₂lc := A₂ki.TypeVarLocallyClosed_of
+          rw [A₂lc.weaken (n := 1) |>.TypeVar_open_eq, A₂lc.TypeVar_open_eq, ← Δ.empty_append]
+          apply A₂ki.weakening (Δ' := .empty) (Δ'' := .typeExt (.typeExt .empty a _) aₜ _)
+          rw [Environment.empty_append]
+          exact Δwf.typeVarExt anin |>.typeVarExt aₜnin
+      · exact var .head
+
+theorem ind_evidence (Δwf : [[⊢ Δ]])
+  (Bᵣki : [[Δ, aₗ : *, aₜ : K, aₚ : L K, aᵢ : L K, aₙ : L K ⊢ Bᵣ^aₙ^aᵢ^aₚ^aₜ^aₗ : *]])
+  (Bₗki : [[Δ, aᵢ : L K, aₙ : L K ⊢ Bₗ^aₙ^aᵢ : *]])
+  : [[Δ ⊢ ∀ aₘ : (L K) ↦ *. (∀ aₗ : *. ∀ aₜ : K. ∀ aₚ : L K. ∀ aᵢ : L K. ∀ aₙ : L K. Bᵣ → Bₗ → aₗ$4 → aₘ$5 aₚ$2 → aₘ$5 aₙ$0) → aₘ$5 { } → aₘ$5 A : *]] := sorry
+
+end «F⊗⊕ω».Kinding
+
+mutual
+
+@[simp]
+theorem TypeLambda.TypeVar_open_sizeOf («λτ» : TypeLambda)
+  : sizeOf («λτ».TypeVar_open a n) = sizeOf «λτ» := open TypeLambda in by
+  let .mk κ τ := «λτ»
+  rw [TypeVar_open, mk.sizeOf_spec, mk.sizeOf_spec, τ.TypeVar_open_sizeOf]
+
+@[simp]
+theorem Monotype.TypeVar_open_sizeOf (τ : Monotype) : sizeOf (τ.TypeVar_open a n) = sizeOf τ :=
+  open Monotype in by
+  match τ with
+  | .var (.bound _) =>
+    rw [TypeVar_open]
+    split
+    · case isTrue h =>
+      rw [var.sizeOf_spec, var.sizeOf_spec, ← h]
+      dsimp only [sizeOf]
+      rw [default.sizeOf, default.sizeOf]
+    · case isFalse => rfl
+  | .var (.free _) =>
+    rw [TypeVar_open]
+    split <;> rfl
+  | .app φ τ =>
+    rw [TypeVar_open, app.sizeOf_spec, app.sizeOf_spec, φ.TypeVar_open_sizeOf,
+        τ.TypeVar_open_sizeOf]
+  | .arr τ₀ τ₁ =>
+    rw [TypeVar_open, arr.sizeOf_spec, arr.sizeOf_spec, τ₀.TypeVar_open_sizeOf,
+        τ₁.TypeVar_open_sizeOf]
+  | .label _ => rw [TypeVar_open]
+  | .floor ξ => rw [TypeVar_open, floor.sizeOf_spec, floor.sizeOf_spec, ξ.TypeVar_open_sizeOf]
+  | .comm _ => rw [TypeVar_open]
+  | .row ξτs =>
+    rw [TypeVar_open, List.mapMem_eq_map]
+    match ξτs with
+    | [] => rw [List.map]
+    | (ξ, τ) :: ξτs' =>
+      rw [List.map, row.sizeOf_spec, row.sizeOf_spec, List.cons.sizeOf_spec, List.cons.sizeOf_spec,
+          Prod.mk.sizeOf_spec, Prod.mk.sizeOf_spec, ξ.TypeVar_open_sizeOf, τ.TypeVar_open_sizeOf]
+      have : sizeOf ((row ξτs').TypeVar_open a n) = sizeOf (row ξτs') :=
+        (row ξτs').TypeVar_open_sizeOf
+      rw [TypeVar_open, List.mapMem_eq_map, row.sizeOf_spec, row.sizeOf_spec] at this
+      rw [Nat.add_comm (n := 1) (m := (1 + sizeOf ξ + _)), Nat.add_assoc, this,
+          ← Nat.add_assoc (m := 1), ← Nat.add_comm (n := 1) (m := (1 + sizeOf ξ + _))]
+  | .prod μ ρ =>
+    rw [TypeVar_open, prod.sizeOf_spec, prod.sizeOf_spec, μ.TypeVar_open_sizeOf,
+        ρ.TypeVar_open_sizeOf]
+  | .sum μ ρ =>
+    rw [TypeVar_open, sum.sizeOf_spec, sum.sizeOf_spec, μ.TypeVar_open_sizeOf,
+        ρ.TypeVar_open_sizeOf]
+  | .lift «λτ» ρ =>
+    rw [TypeVar_open, lift.sizeOf_spec, lift.sizeOf_spec, «λτ».TypeVar_open_sizeOf,
+        ρ.TypeVar_open_sizeOf]
+  | .contain ρ₀ μ ρ₁ =>
+    rw [TypeVar_open, contain.sizeOf_spec, contain.sizeOf_spec, ρ₀.TypeVar_open_sizeOf,
+        μ.TypeVar_open_sizeOf, ρ₁.TypeVar_open_sizeOf]
+  | .concat ρ₀ μ ρ₁ ρ₂ =>
+    rw [TypeVar_open, concat.sizeOf_spec, concat.sizeOf_spec, ρ₀.TypeVar_open_sizeOf,
+        μ.TypeVar_open_sizeOf, ρ₁.TypeVar_open_sizeOf, ρ₂.TypeVar_open_sizeOf]
+  | .typeClass _ τ =>
+    rw [TypeVar_open, typeClass.sizeOf_spec, typeClass.sizeOf_spec, τ.TypeVar_open_sizeOf]
+  | .all «λτ» ρ =>
+    rw [TypeVar_open, all.sizeOf_spec, all.sizeOf_spec, «λτ».TypeVar_open_sizeOf,
+        ρ.TypeVar_open_sizeOf]
+  | .ind ρ => rw [TypeVar_open, ind.sizeOf_spec, ind.sizeOf_spec, ρ.TypeVar_open_sizeOf]
+  | .split «λτ» ρ₀ ρ₁ ρ₂ =>
+    rw [TypeVar_open, split.sizeOf_spec, split.sizeOf_spec, «λτ».TypeVar_open_sizeOf,
+        ρ₀.TypeVar_open_sizeOf, ρ₁.TypeVar_open_sizeOf, ρ₂.TypeVar_open_sizeOf]
+
+end
+
+@[simp]
+theorem Monotype.sizeOf_pos (τ : Monotype) : 0 < sizeOf τ := by cases τ <;> simp_arith
+
+mutual
+
+@[simp]
+noncomputable
+def TypeLambda.sizeOf' : TypeLambda → Nat | .mk κ τ => 1 + sizeOf κ + τ.sizeOf'
+
+@[simp]
+noncomputable
+def Monotype.sizeOf' : Monotype → Nat
+  | .var a => 1 + sizeOf a
+  | .app φ τ => 1 + φ.sizeOf' + τ.sizeOf'
+  | .arr τ₀ τ₁ => 1 + τ₀.sizeOf' + τ₁.sizeOf'
+  | .label ℓ => 1 + sizeOf ℓ
+  | .floor ξ => 1 + ξ.sizeOf'
+  | .comm u => 1 + sizeOf u
+  | .row ξτs => 1 + (List.sum <| ξτs.mapMem fun (ξ, τ) _ => ξ.sizeOf' + τ.sizeOf')
+  | .prod μ ρ => 1 + μ.sizeOf' + ρ.sizeOf'
+  | .sum μ ρ => 1 + μ.sizeOf' + ρ.sizeOf'
+  | .lift «λτ» ρ => 1 + «λτ».sizeOf' + ρ.sizeOf'
+  | .contain ρ₀ μ ρ₁ => 1 + ρ₀.sizeOf' + μ.sizeOf' + ρ₁.sizeOf'
+  | .concat ρ₀ μ ρ₁ ρ₂ => 1 + ρ₀.sizeOf' + μ.sizeOf' + ρ₁.sizeOf' + ρ₂.sizeOf'
+  | .typeClass _ τ => 1 + τ.sizeOf'
+  | .all «λτ» ρ => 1 + «λτ».sizeOf' + ρ.sizeOf'
+  | .ind ρ => 14 + ρ.sizeOf'
+  | .split «λτ» ρ₀ ρ₁ ρ₂ => 5 + «λτ».sizeOf' + ρ₀.sizeOf' + ρ₁.sizeOf' + ρ₂.sizeOf'
+
+end
+
+@[simp]
+theorem Monotype.sizeOf'_pos (τ : Monotype) : 0 < τ.sizeOf' := by cases τ <;> simp_arith [sizeOf']
+
+mutual
+
+@[simp]
+theorem TypeLambda.TypeVar_open_sizeOf' («λτ» : TypeLambda)
+  : («λτ».TypeVar_open a n).sizeOf' = «λτ».sizeOf' := open TypeLambda in by
+  let .mk κ τ := «λτ»
+  rw [TypeVar_open, sizeOf', sizeOf', τ.TypeVar_open_sizeOf']
+
+@[simp]
+theorem Monotype.TypeVar_open_sizeOf' (τ : Monotype) : (τ.TypeVar_open a n).sizeOf' = τ.sizeOf' :=
+  open Monotype in by
+  match τ with
+  | .var (.bound _) =>
+    rw [TypeVar_open]
+    split
+    · case isTrue h =>
+      rw [sizeOf', sizeOf', ← h]
+      dsimp only [sizeOf]
+      rw [default.sizeOf, default.sizeOf]
+    · case isFalse => rfl
+  | .var (.free _) =>
+    rw [TypeVar_open]
+    split
+    · case isTrue h =>
+      rw [sizeOf', sizeOf']
+      dsimp only [sizeOf]
+      rw [default.sizeOf, default.sizeOf]
+    · case isFalse h => rfl
+  | .app φ τ =>
+    rw [TypeVar_open, sizeOf', sizeOf', φ.TypeVar_open_sizeOf', τ.TypeVar_open_sizeOf']
+  | .arr τ₀ τ₁ =>
+    rw [TypeVar_open, sizeOf', sizeOf', τ₀.TypeVar_open_sizeOf', τ₁.TypeVar_open_sizeOf']
+  | .label _ => rw [TypeVar_open]
+  | .floor ξ => rw [TypeVar_open, sizeOf', sizeOf', ξ.TypeVar_open_sizeOf']
+  | .comm _ => rw [TypeVar_open]
+  | .row ξτs =>
+    rw [TypeVar_open, List.mapMem_eq_map]
+    match ξτs with
+    | [] => rw [List.map]
+    | (ξ, τ) :: ξτs' =>
+      rw [List.map, sizeOf', sizeOf', List.mapMem_eq_map, List.map_cons, List.sum_cons,
+          ξ.TypeVar_open_sizeOf', τ.TypeVar_open_sizeOf']
+      have : ((row ξτs').TypeVar_open a n).sizeOf' = (row ξτs').sizeOf' :=
+        (row ξτs').TypeVar_open_sizeOf'
+      rw [TypeVar_open, List.mapMem_eq_map, sizeOf', sizeOf', List.mapMem_eq_map] at this
+      rw [← Nat.add_assoc, Nat.add_comm (n := 1), Nat.add_assoc, this, List.mapMem, List.sum_cons,
+          ← Nat.add_assoc, Nat.add_comm (m := 1), Nat.add_assoc]
+  | .prod μ ρ =>
+    rw [TypeVar_open, sizeOf', sizeOf', μ.TypeVar_open_sizeOf', ρ.TypeVar_open_sizeOf']
+  | .sum μ ρ =>
+    rw [TypeVar_open, sizeOf', sizeOf', μ.TypeVar_open_sizeOf', ρ.TypeVar_open_sizeOf']
+  | .lift «λτ» ρ =>
+    rw [TypeVar_open, sizeOf', sizeOf', «λτ».TypeVar_open_sizeOf', ρ.TypeVar_open_sizeOf']
+  | .contain ρ₀ μ ρ₁ =>
+    rw [TypeVar_open, sizeOf', sizeOf', ρ₀.TypeVar_open_sizeOf', μ.TypeVar_open_sizeOf',
+        ρ₁.TypeVar_open_sizeOf']
+  | .concat ρ₀ μ ρ₁ ρ₂ =>
+    rw [TypeVar_open, sizeOf', sizeOf', ρ₀.TypeVar_open_sizeOf', μ.TypeVar_open_sizeOf',
+        ρ₁.TypeVar_open_sizeOf', ρ₂.TypeVar_open_sizeOf']
+  | .typeClass _ τ =>
+    rw [TypeVar_open, sizeOf', sizeOf', τ.TypeVar_open_sizeOf']
+  | .all «λτ» ρ =>
+    rw [TypeVar_open, sizeOf', sizeOf', «λτ».TypeVar_open_sizeOf', ρ.TypeVar_open_sizeOf']
+  | .ind ρ => rw [TypeVar_open, sizeOf', sizeOf', ρ.TypeVar_open_sizeOf']
+  | .split «λτ» ρ₀ ρ₁ ρ₂ =>
+    rw [TypeVar_open, sizeOf', sizeOf', «λτ».TypeVar_open_sizeOf', ρ₀.TypeVar_open_sizeOf',
+        ρ₁.TypeVar_open_sizeOf', ρ₂.TypeVar_open_sizeOf']
+
+end
+namespace QualifiedType
+
+@[simp]
+theorem sizeOf_pos (γ : QualifiedType) : 0 < sizeOf γ := by cases γ <;> simp_arith
+
+@[simp]
+theorem TypeVar_open_sizeOf (γ : QualifiedType) : sizeOf (γ.TypeVar_open a n) = sizeOf γ := by
+  match γ with
+  | .mono τ => rw [TypeVar_open, mono.sizeOf_spec, mono.sizeOf_spec, τ.TypeVar_open_sizeOf]
+  | .qual ψ γ =>
+    rw [TypeVar_open, qual.sizeOf_spec, qual.sizeOf_spec, ψ.TypeVar_open_sizeOf,
+        γ.TypeVar_open_sizeOf]
+
+@[simp]
+noncomputable
+def sizeOf' : QualifiedType → Nat
+  | .mono τ => 1 + τ.sizeOf'
+  | .qual ψ γ => 1 + ψ.sizeOf' + γ.sizeOf'
+
+@[simp]
+theorem sizeOf'_pos (γ : QualifiedType) : 0 < γ.sizeOf' := by cases γ <;> simp_arith [sizeOf']
+
+@[simp]
+theorem TypeVar_open_sizeOf' (γ : QualifiedType) : (γ.TypeVar_open a n).sizeOf' = γ.sizeOf' := by
+  match γ with
+  | .mono τ => rw [TypeVar_open, sizeOf', sizeOf', τ.TypeVar_open_sizeOf']
+  | .qual ψ γ => rw [TypeVar_open, sizeOf', sizeOf', ψ.TypeVar_open_sizeOf', γ.TypeVar_open_sizeOf']
+
+end QualifiedType
+
+theorem ClassEnvironment.WellFormedness.ext_eliml (Γcγcw : [[⊢c Γc, γc]]) : [[⊢c Γc]] :=
+  let .ext Γcw .. := Γcγcw
+  Γcw
+
+namespace TypeScheme
+
+@[simp]
+theorem TypeVar_open_sizeOf (σ : TypeScheme) : sizeOf (σ.TypeVar_open a n) = sizeOf σ := by
+  match σ with
+  | .qual γ => rw [TypeVar_open, qual.sizeOf_spec, qual.sizeOf_spec, γ.TypeVar_open_sizeOf]
+  | .quant _ σ => rw [TypeVar_open, quant.sizeOf_spec, quant.sizeOf_spec, σ.TypeVar_open_sizeOf]
+
+@[simp]
+noncomputable
+def sizeOf' : TypeScheme → Nat
+  | .qual γ => 1 + γ.sizeOf'
+  | .quant _ σ => 2 + σ.sizeOf'
+
+@[simp]
+theorem sizeOf'_pos (σ : TypeScheme) : 0 < σ.sizeOf' := by cases σ <;> simp_arith [sizeOf']
+
+@[simp]
+theorem TypeVar_open_sizeOf' (σ : TypeScheme) : (σ.TypeVar_open a n).sizeOf' = σ.sizeOf' := by
+  match σ with
+  | .qual γ => rw [TypeVar_open, sizeOf', sizeOf', γ.TypeVar_open_sizeOf']
+  | .quant _ σ => rw [TypeVar_open, sizeOf', sizeOf', σ.TypeVar_open_sizeOf']
+
+theorem of_ClassEnvironmentWellFormedness_of_ClassEnvironment_in {TC} (Γcw : [[⊢c Γc]])
+  (TCin : [[(</ TCₛ@i a ⇝ Aₛ@i // i ∈ [:n] /> ⇒ TC a : κ) ↦ m : σ ⇝ A ∈ Γc]]) (κe : [[⊢ κ ⇝ K]])
+  : ∀ a, [[ε, a : K ⊢ A^a : *]] ∧ ∀ i ∈ [:n], [[ε, a : K ⊢ Aₛ@i^a : *]] := by
+  intro a
+  generalize γceq : ClassEnvironmentEntry.mk
+    (List.map (fun i => [(TCₛ i, Aₛ i)]) (Coe.coe [:n])).flatten TC κ m σ A = γc at TCin
+  match TCin with
+  | .head =>
+    let .ext _ κ'e _ Aopki _ Aₛopki := Γcw
+    let ⟨TCₛAₛeq, _, κeqκ', _, _, AeqA'⟩ := ClassEnvironmentEntry.mk.inj γceq
+    cases κeqκ'
+    cases AeqA'
+    cases κe.deterministic κ'e
+    exact ⟨
+      Aopki a,
+      fun i inin => by
+        rw [List.map_singleton_flatten, List.map_singleton_flatten] at TCₛAₛeq
+        let length_eq : List.length (List.map _ _) = List.length _ := by rw [TCₛAₛeq]
+        dsimp [Coe.coe] at length_eq
+        rw [List.length_map, List.length_map, Std.Range.length_toList, Std.Range.length_toList,
+            Nat.sub_zero, Nat.sub_zero] at length_eq
+        cases length_eq
+        rw [And.right <| Prod.mk.inj <| Std.Range.eq_of_mem_of_map_eq' TCₛAₛeq i inin]
+        exact Aₛopki i inin a
+    ⟩
+  | .ext TCin' .. =>
+    let ⟨TCₛAₛeq, _, κeqκ', _, _, AeqA'⟩ := ClassEnvironmentEntry.mk.inj γceq
+    cases κeqκ'
+    cases AeqA'
+    let ⟨Aopki, Aₛopki⟩ :=
+      of_ClassEnvironmentWellFormedness_of_ClassEnvironment_in Γcw.ext_eliml TCin' κe a
+    exact ⟨
+      Aopki,
+      fun i inin => by
+        rw [List.map_singleton_flatten, List.map_singleton_flatten] at TCₛAₛeq
+        let length_eq : List.length (List.map _ _) = List.length _ := by rw [TCₛAₛeq]
+        dsimp [Coe.coe] at length_eq
+        rw [List.length_map, List.length_map, Std.Range.length_toList, Std.Range.length_toList,
+            Nat.sub_zero, Nat.sub_zero] at length_eq
+        cases length_eq
+        rw [And.right <| Prod.mk.inj <| Std.Range.eq_of_mem_of_map_eq' TCₛAₛeq i inin]
+        exact Aₛopki i inin
+    ⟩
+
+end TypeScheme
+
+namespace TypeEnvironment
+
+@[simp]
+noncomputable
+def sizeOf' : TypeEnvironment → Nat
+  | .empty => 1
+  | .typeExt Γ _ _ => 1 + Γ.sizeOf'
+  | .termExt Γ _ σ => 1 + Γ.sizeOf' + σ.sizeOf'
+  | .constrExt Γ ψ _ => 3 + Γ.sizeOf' + ψ.sizeOf'
+
+namespace WellFormednessAndElaboration
+
+theorem TypeVarNotInDom_preservation (Γwe : [[Γc ⊢ Γ ⇝ Δ]]) (anin : [[a ∉ dom(Γ)]])
+  : [[a ∉ dom(Δ)]] := fun ainΔ => match Γwe with
+  | .empty => nomatch ainΔ
+  | .typeExt Γ'we .. => match List.mem_cons.mp ainΔ with
+    | .inl (.refl _) => anin <| .head _
+    | .inr ainΔ' => Γ'we.TypeVarNotInDom_preservation (List.not_mem_of_not_mem_cons anin) ainΔ'
+  | .termExt Γ'we .. | .constrExt Γ'we .. => Γ'we.TypeVarNotInDom_preservation anin ainΔ
+
+theorem TermVarNotInDom_preservation (Γwe : [[Γc ⊢ Γ ⇝ Δ]]) (xnin : [[x ∉ dom'(Γ)]])
+  : [[x ∉ dom(Δ)]] := fun xinΔ => match Γwe with
+  | .empty => nomatch xinΔ
+  | .typeExt Γ'we .. => Γ'we.TermVarNotInDom_preservation xnin xinΔ
+  | .termExt Γ'we .. | .constrExt Γ'we .. => match List.mem_cons.mp xinΔ with
+    | .inl (.refl _) => xnin <| .head _
+    | .inr xinΔ' => Γ'we.TermVarNotInDom_preservation (List.not_mem_of_not_mem_cons xnin) xinΔ'
+
+end WellFormednessAndElaboration
+
+end TypeEnvironment
+
+mutual
+
+theorem TypeScheme.KindingAndElaboration.soundness (σke : [[Γc; Γ ⊢ σ : κ ⇝ A]])
+  (Γwe : [[Γc ⊢ Γ ⇝ Δ]]) (κe : [[⊢ κ ⇝ K]]) : [[Δ ⊢ A : K]] := open TypeScheme in match σ, σke with
+  | .qual (.mono (.var _)), .var aκinΓ => .var <| Γwe.TypeVarIn_preservation aκinΓ κe
+  | .qual (.mono (.app φ τ)), .app φke τke (κ₀ := κ₀) =>
+    let ⟨K₀, κ₀e⟩ := κ₀.Elaboration_total
+    .app (φke.soundness Γwe (.arr κ₀e κe)) (τke.soundness Γwe κ₀e)
+  | .qual (.mono (.arr τ₀ τ₁)), .arr τ₀ke τ₁ke =>
+    let .star := κe
+    .arr (τ₀ke.soundness Γwe .star) (τ₁ke.soundness Γwe .star)
+  | .quant κ' σ', .scheme I σ'ke κ'e =>
+    .scheme (I := Γ.typeVarDom ++ I) fun a anin =>
+      let ⟨aninΓ, aninI⟩ := List.not_mem_append'.mp anin
+      σ'ke a aninI |>.soundness (Γwe.typeExt aninΓ κ'e) κe
+  | .qual (.qual ψ γ), .qual φke γke κe' => by
+    cases κe.deterministic κe'
+    exact .arr (φke.soundness Γwe .constr) (γke.soundness Γwe κe')
+  | .qual (.mono (.label _)), .label => let .label := κe; .unit
+  | .qual (.mono (.floor _)), .floor _ => let .star := κe; .unit
+  | .qual (.mono (.comm _)), .comm => let .comm := κe; .unit
+  | .qual (.mono (.row ..)), .row _ _ τke =>
+    let .row κ'e := κe
+    .list fun i imem => τke i imem |>.soundness Γwe κ'e
+  | .qual (.mono (.prod μ ρ)), .prod μke ρke =>
+    let .star := κe
+    .prod <| ρke.soundness Γwe <| .row .star
+  | .qual (.mono (.sum μ ρ)), .sum μke ρke =>
+    let .star := κe
+    .sum <| ρke.soundness Γwe <| .row .star
+  | .qual (.mono (.lift (.mk κ' τ) ρ)), σke =>
+    let .row κ₁e := κe
+    let .lift I τke κ₀e ρke := σke
+    let Aopki : «F⊗⊕ω».Kinding .. := .lam (I := Γ.typeVarDom ++ I) fun a anin =>
+      let ⟨aninΓ, aninI⟩ := List.not_mem_append'.mp anin
+      τke a aninI |>.soundness (Γwe.typeExt aninΓ κ₀e) κ₁e
+    .listApp Aopki (ρke.soundness Γwe κ₀e.row)
+  | .qual (.mono (.contain ρ₀ μ ρ₁)), .contain _ ρ₀ke ρ₁ke κ'e (K := K') (A₀ := A₀) (A₁ := A₁) => by
+    let .constr := κe
+    apply Kinding.prod
+    let A i : «Type» := match i with
+      | 0 => [[∀ a : K' ↦ *. (⊗ (a$0 ⟦A₁⟧)) → ⊗ (a$0 ⟦A₀⟧)]]
+      | 1 => [[∀ a : K' ↦ *. (⊕ (a$0 ⟦A₀⟧)) → ⊕ (a$0 ⟦A₁⟧)]]
+      | _ => .list []
+    let Δwf := Γwe.soundness
+    let A₀k := ρ₀ke.soundness Γwe κ'e.row
+    let A₁k := ρ₁ke.soundness Γwe κ'e.row
+    have := Kinding.list (Δ := Δ) (A := A) (K := .star) (n := 2)
+      fun | 0, _ => .prj_evidence Δwf A₀k A₁k | 1, _ => .inj_evidence Δwf A₀k A₁k
+    simp [Coe.coe, Std.Range.toList, A] at this
+    exact this
+  | .qual (.mono (.concat ρ₀ μ ρ₁ ρ₂)), .concat _ ρ₀ke ρ₁ke ρ₂ke κ'e containl containr (K := K')
+      (A₀ := A₀) (A₁ := A₁) (A₂ := A₂) (Bₗ := Bₗ) (Bᵣ := Bᵣ) => by
+    let .constr := κe
+    apply Kinding.prod
+    let A i : «Type» := match i with
+      | 0 => [[∀ a : K' ↦ *. (⊗ (a$0 ⟦A₀⟧)) → (⊗ (a$0 ⟦A₁⟧)) → ⊗ (a$0 ⟦A₂⟧)]]
+      | 1 => [[∀ a : K' ↦ *. ∀ aₜ : *. ((⊕ (a$1 ⟦A₀⟧)) → aₜ$0) → ((⊕ (a$1 ⟦A₁⟧)) → aₜ$0) → (⊕ (a$1 ⟦A₂⟧)) → aₜ$0]]
+      | 2 => Bₗ
+      | 3 => Bᵣ
+      | _ => .list []
+    let Δwf := Γwe.soundness
+    let A₀k := ρ₀ke.soundness Γwe κ'e.row
+    let A₁k := ρ₁ke.soundness Γwe κ'e.row
+    let A₂k := ρ₂ke.soundness Γwe κ'e.row
+    have := Kinding.list (Δ := Δ) (A := A) (K := .star) (n := 4)
+      fun
+        | 0, _ => .concat_evidence Δwf A₀k A₁k A₂k
+        | 1, _ => .elim_evidence Δwf A₀k A₁k A₂k
+        | 2, _ => containl.soundness Γwe .constr
+        | 3, _ => containr.soundness Γwe .constr
+    simp [Coe.coe, Std.Range.toList, A] at this
+    exact this
+  | .qual (.mono (.typeClass _ τ)),
+    .tc Γcw inΓc τke (κ := κ') (A := A') (Aₛ := Aₛ) (B := B) (n := n) => by
+    let .constr := κe
+    apply Kinding.prod
+    let A'' i := if i = 0 then A'.Type_open B else (Aₛ (i - 1)).Type_open B
+    have := Kinding.list (Δ := Δ) (n := n + 1) (A := A'') (K := .star) ?h
+    rw [List.map_singleton_flatten] at *
+    dsimp only [Coe.coe] at this
+    rw [Std.Range.toList, if_neg (nomatch ·), if_pos (Nat.zero_lt_succ _), List.map] at this
+    simp only at this
+    dsimp only [A''] at this
+    rw [if_pos rfl, ← Std.Range.map_shift (Nat.le_refl 1), Nat.sub_self, Nat.add_sub_cancel] at this
+    exact this
+    intro i ⟨_, iltnsucc⟩
+    dsimp only [A'']
+    let ⟨K', κ'e⟩ := κ'.Elaboration_total
+    let Bk := τke.soundness Γwe κ'e
+    split
+    · case isTrue h =>
+      let ⟨a, anin⟩ := Γ.typeVarDom ++ ↑A'.fv |>.exists_fresh
+      let ⟨aninΓ, aninA'⟩ := List.not_mem_append'.mp anin
+      let ⟨A'k, _⟩ := of_ClassEnvironmentWellFormedness_of_ClassEnvironment_in Γcw inΓc κ'e a
+      exact A'k.weakening (Γwe.soundness.typeVarExt <| Γwe.TypeVarNotInDom_preservation aninΓ)
+        (Δ'' := .empty) |>.Type_open_preservation (Δ' := .empty) aninA' Bk
+    · case isFalse h =>
+      let ⟨a, anin⟩ := Γ.typeVarDom ++ ↑(Aₛ (i - 1)).fv |>.exists_fresh
+      let ⟨aninΓ, aninAₛ⟩ := List.not_mem_append'.mp anin
+      let ⟨_, Aₛke⟩ := of_ClassEnvironmentWellFormedness_of_ClassEnvironment_in Γcw inΓc κ'e a
+      rw [Nat.add_comm] at iltnsucc
+      have : i - 1 < n := Nat.sub_lt_left_of_lt_add (Nat.pos_of_ne_zero h) iltnsucc
+      exact Aₛke (i - 1) ⟨Nat.zero_le _, this⟩
+        |>.weakening (Γwe.soundness.typeVarExt <| Γwe.TypeVarNotInDom_preservation aninΓ)
+          (Δ'' := .empty) |>.Type_open_preservation (Δ' := .empty) aninAₛ Bk
+  | .qual (.mono (.all (.mk κ ψ) ρ)), .all I ψke κe' ρke =>
+    let .constr := κe
+    let Aopki : «F⊗⊕ω».Kinding .. := .lam (I := Γ.typeVarDom ++ I) fun a anin =>
+      let ⟨aninΓ, aninI⟩ := List.not_mem_append'.mp anin
+      ψke a aninI |>.soundness (Γwe.typeExt aninΓ κe') .constr
+    .prod <| .listApp Aopki <| ρke.soundness Γwe κe'.row
+  | .qual (.mono (.ind ρ)), .ind I₀ I₁ ρke κ'e Bᵣke Bₗke =>
+    let .constr := κe
+    let ⟨aₗ, aₗnin⟩ := Γ.typeVarDom ++ I₀ |>.exists_fresh
+    let ⟨aₗninΓ, aₗnin₀⟩ := List.not_mem_append'.mp aₗnin
+    let Γₗ := Γ.typeExt aₗ _
+    let I₀ₗ : List TypeVarId := aₗ :: I₀
+    let ⟨aₜ, aₜnin⟩ := Γₗ.typeVarDom ++ I₀ₗ |>.exists_fresh
+    let ⟨aₜninΓ, aₜnin₀⟩ := List.not_mem_append'.mp aₜnin
+    let Γₗₜ := Γₗ.typeExt aₜ _
+    let I₀ₗₜ : List TypeVarId := aₜ :: I₀ₗ
+    let ⟨aₚ, aₚnin⟩ := Γₗₜ.typeVarDom ++ I₀ₗₜ |>.exists_fresh
+    let ⟨aₚninΓ, aₚnin₀⟩ := List.not_mem_append'.mp aₚnin
+    let Γₗₜₚ := Γₗₜ.typeExt aₚ _
+    let I₀ₗₜₚ : List TypeVarId := aₚ :: I₀ₗₜ
+    let ⟨aᵢ, aᵢnin⟩ := Γₗₜₚ.typeVarDom ++ I₀ₗₜₚ ++ I₁ |>.exists_fresh
+    let ⟨aᵢninΓₗₜₚ₀, aᵢnin₁⟩ := List.not_mem_append'.mp aᵢnin
+    let ⟨aᵢninΓₗₜₚ, aᵢnin₀⟩ := List.not_mem_append'.mp aᵢninΓₗₜₚ₀
+    let aᵢninΓ := List.not_mem_of_not_mem_cons <| List.not_mem_of_not_mem_cons
+      <| List.not_mem_of_not_mem_cons <| aᵢninΓₗₜₚ
+    let Γₗₜₚᵢ := Γₗₜₚ.typeExt aᵢ _
+    let I₀ₗₜₚᵢ : List TypeVarId := aᵢ :: I₀ₗₜₚ
+    let I₁ᵢ : List TypeVarId := aᵢ :: I₁
+    let ⟨aₙ, aₙnin⟩ := Γₗₜₚᵢ.typeVarDom ++ I₀ₗₜₚᵢ ++ I₁ᵢ |>.exists_fresh
+    let ⟨aₙninΓₗₜₚᵢ₀, aₙnin₁⟩ := List.not_mem_append'.mp aₙnin
+    let ⟨aₙninΓₗₜₚᵢ, aₙnin₀⟩ := List.not_mem_append'.mp aₙninΓₗₜₚᵢ₀
+    let ⟨aₙneaᵢ, aₙninΓₗₜₚ⟩ := List.ne_and_not_mem_of_not_mem_cons aₙninΓₗₜₚᵢ
+    let aₙninΓ := List.not_mem_of_not_mem_cons <| List.not_mem_of_not_mem_cons
+      <| List.not_mem_of_not_mem_cons <| aₙninΓₗₜₚ
+    let aₙninΓᵢ := List.not_mem_cons_of_ne_of_not_mem aₙneaᵢ aₙninΓ
+    let Γₗₜₚᵢₙwe := Γwe.typeExt aₗninΓ .label |>.typeExt aₜninΓ κ'e |>.typeExt aₚninΓ κ'e.row
+      |>.typeExt aᵢninΓₗₜₚ κ'e.row |>.typeExt aₙninΓₗₜₚᵢ κ'e.row
+    let Γᵢₙwe := Γwe.typeExt aᵢninΓ κ'e.row |>.typeExt aₙninΓᵢ κ'e.row
+    .ind_evidence Γwe.soundness
+      (Bᵣke aₗ aₗnin₀ aₜ aₜnin₀ aₚ aₚnin₀ aᵢ aᵢnin₀ aₙ aₙnin₀ |>.soundness Γₗₜₚᵢₙwe .constr)
+      (Bₗke aᵢ aᵢnin₁ aₙ aₙnin₁ |>.soundness Γᵢₙwe .constr)
+  | .qual (.mono (.split «λτ» ρ₀ ρ₁ ρ₂)), σke =>
+    let .split concatke := σke
+    concatke.soundness Γwe κe
+termination_by Γ.sizeOf' + σ.sizeOf'
+decreasing_by
+  all_goals simp_arith [List.mapMem]
+  · case _ ξ _ τ _ _ _ _ _ _ =>
+    apply Nat.le_trans <| Nat.le_add_left (τ i).sizeOf' (ξ i).sizeOf'
+    apply List.le_sum_of_mem
+    rw [List.map_singleton_flatten, List.mapMem_eq_map, List.map_map]
+    exact Std.Range.mem_map_of_mem imem
+  · exact Nat.succ_le_of_lt <| Monotype.sizeOf'_pos _
+
+theorem TypeEnvironment.WellFormednessAndElaboration.soundness (Γwe : [[Γc ⊢ Γ ⇝ Δ]]) : [[⊢ Δ]] :=
+  match Γwe with
+  | .empty => .empty
+  | .typeExt Γ'we anin κe => Γ'we.soundness.typeVarExt <| Γ'we.TypeVarNotInDom_preservation anin
+  | .termExt Γ'we xnin σke =>
+    Γ'we.soundness.termVarExt (Γ'we.TermVarNotInDom_preservation xnin) (σke.soundness Γ'we .star)
+  | .constrExt Γ'we xnin ψke =>
+    Γ'we.soundness.termVarExt (Γ'we.TermVarNotInDom_preservation xnin) (ψke.soundness Γ'we .constr)
+termination_by Γ.sizeOf'
+
+end
 
 end TabularTypeInterpreter
